library/init/data/list/lemmas.lean
@@ -192,7 +192,7 @@ theorem length_remove_nth : ∀ (l : list α) (i : ℕ), i < length l → length
 
 @[simp] lemma partition_eq_filter_filter (p : α → Prop) [decidable_pred p] : ∀ (l : list α), partition p l = (filter p l, filter (not ∘ p) l)
 | []     := rfl
-| (a::l) := by { by_cases p a with pa; simp [partition, filter, pa, partition_eq_filter_filter l],
+| (a::l) := by { by_cases pa : p a; simp [partition, filter, pa, partition_eq_filter_filter l],
                  rw [if_neg (not_not_intro pa)], rw [if_pos pa] }
 
 /- sublists -/
@@ -223,7 +223,7 @@ lemma length_le_of_sublist : ∀ {l₁ l₂ : list α}, l₁ <+ l₂ → length 
 @[simp] theorem filter_append {p : α → Prop} [h : decidable_pred p] :
   ∀ (l₁ l₂ : list α), filter p (l₁++l₂) = filter p l₁ ++ filter p l₂
 | []      l₂ := rfl
-| (a::l₁) l₂ := by by_cases p a with pa; simp [pa, filter_append]
+| (a::l₁) l₂ := by by_cases pa : p a; simp [pa, filter_append]
 
 @[simp] theorem filter_sublist {p : α → Prop} [h : decidable_pred p] : Π (l : list α), filter p l <+ l
 | []     := sublist.slnil
