library/init/data/nat/bitwise.lean
@@ -210,21 +210,23 @@ lemma binary_rec_eq {C : nat → Sort u} {z : C 0} {f : ∀ b n, C n → C (bit 
   binary_rec z f (bit b n) = f b n (binary_rec z f n) :=
 begin
   rw [binary_rec],
-  by_cases (bit b n = 0) with h',
-  {simp [dif_pos h'],
-   generalize : binary_rec._main._pack._proof_1 (bit b n) h' = e,
-   revert e,
-   have bf := bodd_bit b n,
-   have n0 := div2_bit b n,
-   rw h' at bf n0,
-   simp at bf n0,
-   rw [← bf, ← n0, binary_rec_zero],
-   intros, exact h.symm },
-  {simp [dif_neg h'],
-   generalize : binary_rec._main._pack._proof_2 (bit b n) = e,
-   revert e,
-   rw [bodd_bit, div2_bit],
-   intros, refl}
+  with_cases { by_cases bit b n = 0 },
+  case pos : h' {
+    simp [dif_pos h'],
+    generalize : binary_rec._main._pack._proof_1 (bit b n) h' = e,
+    revert e,
+    have bf := bodd_bit b n,
+    have n0 := div2_bit b n,
+    rw h' at bf n0,
+    simp at bf n0,
+    rw [← bf, ← n0, binary_rec_zero],
+    intros, exact h.symm },
+  case neg : h' {
+    simp [dif_neg h'],
+    generalize : binary_rec._main._pack._proof_2 (bit b n) = e,
+    revert e,
+    rw [bodd_bit, div2_bit],
+    intros, refl}
 end
 
 lemma bitwise_bit_aux {f : bool → bool → bool} (h : f ff ff = ff) :
